policy_proof/coq/prov.v
@@ -8,7 +8,7 @@ Inductive prov_type: Set :=
   | prov_trans_unary: UnOp → prov_type
   | prov_trans_binary: BinOp → prov_type
   | prov_agg: AggOp -> prov_type
-  | prov_noise: prov_type
+  | prov_noise: NoiseOp → prov_type
   | prov_join: prov_type
 .
 
